src/Init/Data/Iterators/PostconditionMonad.lean
@@ -54,7 +54,7 @@ def PostconditionT.lift {α : Type w} {m : Type w → Type w'} [Functor m] (x : 
   ⟨fun _ => True, (⟨·, .intro⟩) <$> x⟩
 
 @[always_inline, inline, expose]
-def PostconditionT.attachLift {α : Type w} {m : Type w → Type w'} [Functor m] [MonadAttach m]
+def PostconditionT.attachLift {α : Type w} {m : Type w → Type w'} [MonadAttach m]
     (x : m α) : PostconditionT m α :=
   ⟨MonadAttach.CanReturn x, MonadAttach.attach x⟩
 
@@ -120,6 +120,11 @@ Converts an operation from `PostConditionT m` to `m`, discarding the postconditi
 def PostconditionT.run {m : Type w → Type w'} [Monad m] {α : Type w} (x : PostconditionT m α) :
     m α :=
   (fun a => a.val) <$> x.operation
+
+theorem PostconditionT.run_eq_map {m : Type w → Type w'} [Monad m] {α : Type w}
+    {x : PostconditionT m α} :
+    x.run = Subtype.val <$> x.operation :=
+  (rfl)
 
 instance {m : Type w → Type w'} [Functor m] : Functor (PostconditionT m) where
   map := PostconditionT.map
@@ -243,6 +248,28 @@ theorem PostconditionT.operation_bind' {m : Type w → Type w'} [Monad m] {α : 
       (fun fa => ⟨fa.1, by exact⟨a.1, a.2, fa.2⟩⟩) <$> (f a.1).operation) := by
   rfl
 
+theorem PostconditionT.operation_eq_map_mk_operation {m : Type w → Type w'}
+    [Monad m] [LawfulMonad m] {x : PostconditionT m α} :
+    x.operation = (fun a => ⟨a.val, a.property⟩) <$> x.operation := by
+  simp
+
+theorem PostconditionT.operation_bind_eq_operation_bind_mk {m : Type w → Type w'}
+    [Monad m] {x : PostconditionT m α} {f : Subtype x.Property → m β} :
+    x.operation >>= f = x.operation >>= (fun a => f ⟨a.val, a.property⟩) := by
+  rfl
+
+@[simp]
+theorem PostconditionT.run_bind {m : Type w → Type w'} [Monad m] [LawfulMonad m]
+    {α : Type w} {β : Type w} {x : PostconditionT m α} {f : α → PostconditionT m β} :
+    (x.bind f).run = x.run >>= (f · |>.run) := by
+  simp [run_eq_map]
+
+@[simp]
+theorem PostconditionT.run_bind' {m : Type w → Type w'} [Monad m] [LawfulMonad m]
+    {α : Type w} {β : Type w} {x : PostconditionT m α} {f : α → PostconditionT m β} :
+    (x >>= f).run = x.run >>= (f · |>.run) :=
+  run_bind
+
 @[simp]
 theorem PostconditionT.property_lift {m : Type w → Type w'} [Functor m] {α : Type w}
     {x : m α} : (lift x : PostconditionT m α).Property = (fun _ => True) := by
@@ -253,6 +280,12 @@ theorem PostconditionT.operation_lift {m : Type w → Type w'} [Functor m] {α :
     {x : m α} : (lift x : PostconditionT m α).operation =
       (⟨·, property_lift (m := m) ▸ True.intro⟩) <$> x := by
   rfl
+
+@[simp]
+theorem PostconditionT.run_attachLift {m : Type w → Type w'} [Monad m] [MonadAttach m]
+    [WeaklyLawfulMonadAttach m] {α : Type w}
+    {x : m α} : (attachLift x).run = x := by
+  simp [attachLift, run_eq_map, WeaklyLawfulMonadAttach.map_attach]
 
 instance {m : Type w → Type w'} {n : Type w → Type w''} [MonadLift m n] :
     MonadLift (PostconditionT m) (PostconditionT n) where
