src/Init/Control/Lawful/MonadAttach/Lemmas.lean
@@ -81,3 +81,10 @@ public theorem WeaklyLawfulMonadAttach.pbind_eq_bind
     MonadAttach.pbind x (fun a _ => f a) = x >>= f := by
   conv => rhs; rw [← map_attach (x := x)]
   simp [MonadAttach.pbind]
+
+public theorem WeaklyLawfulMonadAttach.pbind_eq_bind'
+    [Monad m] [MonadAttach m] [LawfulMonad m] [WeaklyLawfulMonadAttach m]
+    {x : m α} {f : α → m β} :
+    MonadAttach.pbind x (fun a _ => f a) = x >>= f := by
+  conv => rhs; rw [← map_attach (x := x)]
+  simp [MonadAttach.pbind]
